Finite domain heaps model

src/Iris/Algebra/Lib/FiniteHeaps.lean
@@ -15,37 +15,172 @@ inductive FiniteDomFunction (V : Type _)
 | set : Nat → V → FiniteDomFunction V → FiniteDomFunction V
 | remove : Nat → FiniteDomFunction V → FiniteDomFunction V
 
-def FiniteDomFunction.lookup (f : FiniteDomFunction V) (k : Nat) : Option V :=
+open FiniteDomFunction
+
+@[simp] def FiniteDomFunction.lookup (f : FiniteDomFunction V) (k : Nat) : Option V :=
   match f with
   | .empty => none
   | .set n v' rest => if n = k then some v' else rest.lookup k
   | .remove n rest => if n = k then none else rest.lookup k
 
-def FiniteDomFunction.update (f : FiniteDomFunction V) (k : Nat) (v : Option V) : FiniteDomFunction V :=
+@[simp] def FiniteDomFunction.update (f : FiniteDomFunction V) (k : Nat) (v : Option V) : FiniteDomFunction V :=
   match v with
   | some v' => f.set k v'
   | none => f.remove k
 
-instance instFiniteDomStore : Store (FiniteDomFunction V) Nat (Option V) where
-  get := FiniteDomFunction.lookup
-  set := FiniteDomFunction.update
-  merge := sorry
-  get_set_eq := sorry
-  get_set_ne := sorry
-  get_merge := sorry
+@[simp] def FiniteDomFunction.map (F : Nat → V → Option V') (f : FiniteDomFunction V)  : FiniteDomFunction V' :=
+  match f with
+  | .empty => .empty
+  | .set n v rest =>
+      match (F n v) with
+      | .some r => .set n r (rest.map F)
+      | .none => .remove n (rest.map F)
+  | .remove n rest => .remove n (rest.map F)
 
-instance instFiniteDomHeap : Heap (fun V => FiniteDomFunction V) Nat where
-  hmap h f := sorry
-  hmap_alloc := sorry
-  hmap_unalloc := sorry
-  empty _ := sorry
-  get_empty := sorry
+@[simp] def FiniteDomFunction.fresh (f : FiniteDomFunction V) : Nat :=
+  match f with
+  | .empty => 0
+  | .set n _ rest => max (n + 1) rest.fresh
+  | .remove n rest => max (n + 1) rest.fresh
+
+@[simp] def FiniteDomFunction.construct (f : Nat → Option V) (N : Nat) : FiniteDomFunction V :=
+  match N with
+  | .zero => .empty
+  | .succ N' =>
+      match (f N') with
+      | some v => .set N' v (FiniteDomFunction.construct f N')
+      | none => (FiniteDomFunction.construct f N')
+
+@[simp] def FiniteDomFunction.construct_spec (f : Nat → Option V) (N : Nat) : Nat → (Option V) :=
+  fun n => if n < N then f n else none
+
+theorem FiniteDomFunction.lookup_update (f : FiniteDomFunction V):
+    (f.update k v).lookup = fset (f.lookup) k v := by
+  refine funext (fun k' => ?_)
+  cases f <;> cases v <;> simp [fset]
+
+theorem FiniteDomFunction.fresh_lookup_ge (f : FiniteDomFunction V) n :
+    f.fresh ≤ n → f.lookup n = none := by
+  induction f
+  · simp
+  · rename_i n' v' rest IH
+    intro H
+    simp at H
+    simp
+    split <;> rename_i h
+    · omega
+    · apply IH
+      omega
+  · rename_i n' rest IH
+    intro H
+    simp at H
+    simp
+    intro H'
+    apply IH
+    omega
+
+theorem FiniteDomFunction.construct_get (f : Nat → Option V) (N : Nat) :
+    lookup (construct f N) = construct_spec f N := by
+  refine funext (fun k => ?_)
+  rcases Nat.lt_or_ge k N with (HL|HG)
+  · induction N <;> simp
+    rename_i N' IH
+    split <;> rename_i h
+    · simp [h]
+      split
+      · simp_all
+      · rw [IH (by omega)]
+        simp
+        omega
+    · rw [if_pos HL]
+      if h : k < N'
+        then
+          simp [IH h]
+          intro H1
+          omega
+        else
+          have Hx : k = N' := by omega
+          simp_all
+          clear Hx
+          clear h
+          suffices (∀ N'', N' ≤ N'' → (construct f N').lookup N'' = none) by apply this _ N'.le_refl
+          induction N'
+          · simp
+          · rename_i n' IH
+            intro N'' H
+            simp
+            cases h : f n' <;> simp
+            · apply IH
+              omega
+            · split
+              · simp
+                exfalso
+                omega
+              · apply IH
+                omega
+  · simp
+    rw [if_neg (by omega)]
+    induction N <;> simp
+    rename_i N' IH
+    split
+    · simp only [lookup]
+      split; omega
+      apply IH
+      omega
+    · apply IH
+      omega
+instance FiniteDomFunction.instFiniteDomStore : Store (FiniteDomFunction V) Nat (Option V) where
+  get := lookup
+  set := update
+  get_set_eq He := by simp only [lookup_update, fset, if_pos He]
+  get_set_ne He := by simp only [lookup_update, fset, if_neg He]
+
+abbrev op_lift (op : V → V → V) (v1 v2 : Option V) : Option V :=
+  match v1, v2 with
+  | some v1, some v2 => some (op v1 v2)
+  | some v1, none => some v1
+  | none, some v2 => some v2
+  | none, none => none
+
+instance FiniteDomFunction.instFiniteDomHeap : Heap (fun V => FiniteDomFunction V) Nat where
+  hmap h f := f.map h
+  hmap_alloc := by
+    intros V t k v V' f H
+    induction t
+    · simp_all [empty, Store.get, map]
+    · rename_i n' v' t' IH
+      simp_all [Store.get]
+      cases h1 : f n' v' <;> simp <;> split <;> rename_i h2 <;> simp_all
+    · rename_i n' t' IH
+      simp_all [Store.get]
+  hmap_unalloc := by
+    intros V t k V' f H
+    induction t
+    · simp_all [empty, Store.get, map]
+    · rename_i n' v' t' IH
+      simp_all [Store.get]
+      cases h1 : f n' v' <;> simp only [lookup] <;> split <;> simp_all
+    · rename_i n' t' IH
+      simp_all [Store.get]
+  empty _ := .empty
+  get_empty := by intros; simp [Store.get]
+  merge op t1 t2 := construct (fun n => op_lift op (t1.lookup n) (t2.lookup n)) (max t1.fresh t2.fresh)
+  get_merge := by
+    intro V op t1 t2 k
+    simp only [Store.get]
+    simp [FiniteDomFunction.construct_get]
+    split <;> rename_i h
+    · rfl
+    · have Ht1 : t1.fresh ≤ k := by omega
+      have Ht2 : t2.fresh ≤ k := by omega
+      rw [FiniteDomFunction.fresh_lookup_ge _ _ Ht1]
+      rw [FiniteDomFunction.fresh_lookup_ge _ _ Ht2]
 
 instance instFinitDomAllocHeap : AllocHeap (fun V => FiniteDomFunction V) Nat  where
-  notFull f := sorry
-  fresh HC := sorry
-  get_fresh {_ _ HC} := sorry
+  notFull _ := True
+  fresh {_ f} _ := f.fresh
+  get_fresh {_ f _} := fresh_lookup_ge f f.fresh (f.fresh.le_refl)
 
 instance : UnboundedHeap (fun V => FiniteDomFunction V) Nat where
-  notFull_empty := by sorry
-  notFull_set_fresh {V t v H} := by sorry
+  notFull_empty := by simp [notFull]
+  notFull_set_fresh {V t v H} := by simp [notFull]
